# Big O Notation Solutions

## Example 1: Use the definition of O to show that 30nÂ² + 12n + 15 = O(nÂ²)

**Proof:**
We need to find constants c > 0 and nâ‚€ such that 30nÂ² + 12n + 15 â‰¤ cÂ·nÂ² for all n â‰¥ nâ‚€.

For n â‰¥ 1, we have:

- 12n â‰¤ 12nÂ²
- 15 â‰¤ 15nÂ²

Therefore:
30nÂ² + 12n + 15 â‰¤ 30nÂ² + 12nÂ² + 15nÂ² = 57nÂ²

Choose c = 57 and nâ‚€ = 1.
For all n â‰¥ 1: 30nÂ² + 12n + 15 â‰¤ 57nÂ²

Therefore, 30nÂ² + 12n + 15 = O(nÂ²). 

## Example 2: Use the definition of Î© to show that 30nÂ² + 12n + 15 = Î©(nÂ²)

**Proof:**
We need to find constants c > 0 and nâ‚€ such that 30nÂ² + 12n + 15 â‰¥ cÂ·nÂ² for all n â‰¥ nâ‚€.

For n â‰¥ 1:
30nÂ² + 12n + 15 â‰¥ 30nÂ²

Choose c = 30 and nâ‚€ = 1.
For all n â‰¥ 1: 30nÂ² + 12n + 15 â‰¥ 30nÂ²

Therefore, 30nÂ² + 12n + 15 = Î©(nÂ²). 

## Example 3: Use the definition of Î˜ to show that 30nÂ² + 12n + 15 = Î˜(nÂ²)

**Proof:**
By definition, f(n) = Î˜(g(n)) if and only if f(n) = O(g(n)) and f(n) = Î©(g(n)).

From Example 1: 30nÂ² + 12n + 15 = O(nÂ²)
From Example 2: 30nÂ² + 12n + 15 = Î©(nÂ²)

Therefore, 30nÂ² + 12n + 15 = Î˜(nÂ²). 

## Example 4: Use the definition of "big Oh" to show that 2nÂ² - 6n = O(nÂ²)

**Proof:**
We need to find constants c > 0 and nâ‚€ such that 2nÂ² - 6n â‰¤ cÂ·nÂ² for all n â‰¥ nâ‚€.

For n â‰¥ 3, we have nÂ² â‰¥ n, so 6n â‰¤ 6nÂ².
Therefore: 2nÂ² - 6n â‰¤ 2nÂ² - 0 = 2nÂ²

But we need to be more careful. Let's choose nâ‚€ = 3.
For n â‰¥ 3: 6n â‰¤ 2nÂ² (since 6n â‰¤ 2nÂ² when n â‰¥ 3)
Therefore: 2nÂ² - 6n â‰¥ 2nÂ² - 2nÂ² = 0

Actually, let's approach this differently:
2nÂ² - 6n â‰¤ 2nÂ² for all n â‰¥ 1

Choose c = 2 and nâ‚€ = 1.
For all n â‰¥ 1: 2nÂ² - 6n â‰¤ 2nÂ²

Therefore, 2nÂ² - 6n = O(nÂ²). 

## Example 5: Use the definition of "big Omega" to show that 2nÂ² - 6n = Î©(nâ‚€)

**Proof:**
We need to find constants c > 0 and nâ‚€ such that 2nÂ² - 6n â‰¥ cÂ·nâ‚€ for all n â‰¥ nâ‚€.

For large n, the 2nÂ² term dominates, so we need to find when 2nÂ² - 6n â‰¥ cÂ·nâ‚€.

Rearranging: 2nÂ² - 6n â‰¥ cÂ·nâ‚€
2nÂ² - cÂ·nâ‚€ â‰¥ 6n
nâ‚€(2 - c) â‰¥ 6n
nâ‚€(2 - c) â‰¥ 6

Choose c = 1. Then we need nâ‚€(2 - 1) â‰¥ 6, so nâ‚€ â‰¥ 6.
Choose nâ‚€ = 3 (since 3Î© = 9 â‰¥ 6).

For n â‰¥ 3: 2nÂ² - 6n â‰¥ nâ‚€

Therefore, 2nÂ² - 6n = Î©(nâ‚€). 

## Example 6: Conclusion?

From Examples 4 and 5:

- 2nÂ² - 6n = O(nâ‚€)
- 2nÂ² - 6n = Î©(nâ‚€)

Therefore, 2nÂ² - 6n = Î©(nâ‚€).

## Example 7: Find the mistakes in the following "proofs"

**First "proof" mistake:**
The error is using C = -4, which violates the requirement that c > 0. Constants in Big O definitions must be positive.

**Second "proof" mistake:**
Again, C = -4 < 0, which is invalid. Additionally, the inequality 2nÂ² - 6n â‰¥ -4nÂ³ doesn't establish that 2nÂ² - 6n = Î©(nâ‚€), because we need 2nÂ² - 6n â‰¥ cÂ·nâ‚€ for some positive c.

## Example 8, 9 & 10

Beyond the scope of this course. See me in office hours if you'd like to learn more.

---

_Course content developed by Declan Gray-Mullen for WNEU with Claude_
